rocq-bluerock-brick/theories/lang/cpp/logic/atomics.v
@@ -162,7 +162,7 @@ Section with_Σ.
       wrap_shift (fun Q =>
                     Exists v q,  _eqv p |-> primR acc_type q v ** (* pre *)
                                 (_eqv p |-> primR acc_type q v -* Q v)) Q (* post *)
-      |-- wp_atom' AO__atomic_load_n acc_type [p; memorder] Q.
+      |-- wp_atom' "__atomic_load_n" acc_type [p; memorder] Q.
 
   (* An SC store writes the latest value, unless there are racing (no hb)
     non-SC stores. The following rule only holds for SC-only locations. *)
@@ -175,7 +175,7 @@ Section with_Σ.
       [| has_type_prop v acc_type |] **
       wrap_shift (fun Q => _eqv p |-> anyR acc_type (cQp.mut 1) ** (* pre *)
                           (_eqv p |-> primR acc_type (cQp.mut 1) v -* Q Vundef)) Q (* post *)
-      |-- wp_atom' AO__atomic_store_n acc_type [p; memorder; v] Q.
+      |-- wp_atom' "__atomic_store_n" acc_type [p; memorder; v] Q.
 
   (* The following rule holds for SC-only locations, or *no-racing-store*
     locations.
@@ -193,7 +193,7 @@ Section with_Σ.
       wrap_shift (fun Q => Exists w,
                           _eqv p |-> primR acc_type (cQp.mut 1) w ** (* pre *)
                           (_eqv p |-> primR acc_type (cQp.mut 1) v -* Q w)) Q (* post *)
-      |-- wp_atom' AO__atomic_exchange_n acc_type [p; memorder; v] Q.
+      |-- wp_atom' "__atomic_exchange_n" acc_type [p; memorder; v] Q.
 
   (* Again, all of the RMWs rules only read and write latest values if the
     location is SC-only or no-racing-store.
@@ -224,7 +224,7 @@ Section with_Σ.
                   _eqv new_p |-> primR acc_type q new_v **
                   (* ret stores the previous latest value v *)
                   _eqv ret |-> primR acc_type (cQp.mut 1) v -* Q v) >>
-      |-- wp_atom' AO__atomic_exchange acc_type [p; memorder; new_p; ret] Q.
+      |-- wp_atom' "__atomic_exchange" acc_type [p; memorder; new_p; ret] Q.
 
   (* An SC compare and exchange n. This rule combines the postcondition for both
     success and failure case. In the failure case, we know that the values are
@@ -255,7 +255,7 @@ Section with_Σ.
                  \/ b = false /\ v' = v       /\ v <> expected_v |],
             COMM (* post-cond *)
                 _eqv expected_p |-> primR ty (cQp.mut 1) (Vint v) -* Q (Vbool b) >>
-      |-- wp_atom' AO__atomic_compare_exchange_n ty
+      |-- wp_atom' "__atomic_compare_exchange_n" ty
                   [p; succmemord; expected_p; failmemord; Vint desired; weak] Q.
 
   Axiom wp_atom_compare_exchange_n_cst_bool :
@@ -277,7 +277,7 @@ Section with_Σ.
                  \/ b = false /\ v' = v       /\ v <> expected_v |],
             COMM (* post-cond *)
                 _eqv expected_p |-> primR ty (cQp.mut 1) (Vbool v) -* Q (Vbool b) >>
-      |-- wp_atom' AO__atomic_compare_exchange_n ty
+      |-- wp_atom' "__atomic_compare_exchange_n" ty
                   [p; succmemord; expected_p; failmemord; Vbool desired; weak] Q.
 
   (* An SC weak compare exchange. This rule combines the postcondition for both
@@ -306,7 +306,7 @@ Section with_Σ.
                  \/ b = false /\ v' = v |],
             COMM (* post-cond *)
                 _eqv expected_p |-> primR ty (cQp.mut 1) (Vint v) -* Q (Vbool b) >>
-      |-- wp_atom' AO__atomic_compare_exchange_n ty
+      |-- wp_atom' "__atomic_compare_exchange_n" ty
                   [p; succmemord; expected_p; failmemord; Vint desired; weak] Q.
 
   (* TODO: unify with Tnum case *)
@@ -328,7 +328,7 @@ Section with_Σ.
                  \/ b = false /\ v' = v |],
             COMM (* post-cond *)
                 _eqv expected_p |-> primR ty (cQp.mut 1) (Vbool v) -* Q (Vbool b) >>
-      |-- wp_atom' AO__atomic_compare_exchange_n ty
+      |-- wp_atom' "__atomic_compare_exchange_n" ty
                   [p; succmemord; expected_p; failmemord; Vbool desired; weak] Q.
 
   (* TODO: support for pointers, see cpp2v-core#306. *)
@@ -352,7 +352,7 @@ Section with_Σ.
             COMM ((* post-cond *)
                   _eqv expected_p |-> primR ty (cQp.mut 1) (Vint v) **
                   _eqv desired_p |-> primR ty q (Vint desired) -* Q (Vbool b)) >>
-      |-- wp_atom' AO__atomic_compare_exchange ty
+      |-- wp_atom' "__atomic_compare_exchange" ty
                   [p; succmemord; expected_p; failmemord; desired_p; weak] Q.
 
   (* TODO: support for pointers, see cpp2v-core#306. *)
@@ -376,7 +376,7 @@ Section with_Σ.
             COMM ((* post-cond *)
                   _eqv expected_p |-> primR ty (cQp.mut 1) (Vint v) **
                   _eqv desired_p |-> primR ty q (Vint desired) -* Q (Vbool b)) >>
-      |-- wp_atom' AO__atomic_compare_exchange ty
+      |-- wp_atom' "__atomic_compare_exchange" ty
                   [p; succmemord; expected_p; failmemord; desired_p; weak] Q.
 
   (** Atomic operations use two's complement arithmetic. This
@@ -409,12 +409,12 @@ Section with_Σ.
 
   Let nand (a b : Z) : Z := Z.lnot (Z.land a b).
 
-  Axiom wp_atom_fetch_add_cst  : fetch_xxx AO__atomic_fetch_add  Z.add.
-  Axiom wp_atom_fetch_sub_cst  : fetch_xxx AO__atomic_fetch_sub  Z.sub.
-  Axiom wp_atom_fetch_and_cst  : fetch_xxx AO__atomic_fetch_and  Z.land.
-  Axiom wp_atom_fetch_xor_cst  : fetch_xxx AO__atomic_fetch_xor  Z.lxor.
-  Axiom wp_atom_fetch_or_cst   : fetch_xxx AO__atomic_fetch_or   Z.lor.
-  Axiom wp_atom_fetch_nand_cst : fetch_xxx AO__atomic_fetch_nand nand.
+  Axiom wp_atom_fetch_add_cst  : fetch_xxx "__atomic_fetch_add"  Z.add.
+  Axiom wp_atom_fetch_sub_cst  : fetch_xxx "__atomic_fetch_sub"  Z.sub.
+  Axiom wp_atom_fetch_and_cst  : fetch_xxx "__atomic_fetch_and"  Z.land.
+  Axiom wp_atom_fetch_xor_cst  : fetch_xxx "__atomic_fetch_xor"  Z.lxor.
+  Axiom wp_atom_fetch_or_cst   : fetch_xxx "__atomic_fetch_or"   Z.lor.
+  Axiom wp_atom_fetch_nand_cst : fetch_xxx "__atomic_fetch_nand" nand.
 
   (* atomic xxx and fetch rule *)
   Definition wp_xxx_fetch_cst (ao : AtomicOp) (op : Z -> Z -> Z) : Prop :=
@@ -432,12 +432,12 @@ Section with_Σ.
   #[local] Notation xxx_fetch ao op :=
     (Unfold wp_xxx_fetch_cst (wp_xxx_fetch_cst ao op)) (only parsing).
 
-  Axiom wp_atom_add_fetch_cst  : xxx_fetch AO__atomic_add_fetch  Z.add.
-  Axiom wp_atom_sub_fetch_cst  : xxx_fetch AO__atomic_sub_fetch  Z.sub.
-  Axiom wp_atom_and_fetch_cst  : xxx_fetch AO__atomic_and_fetch  Z.land.
-  Axiom wp_atom_xor_fetch_cst  : xxx_fetch AO__atomic_xor_fetch  Z.lxor.
-  Axiom wp_atom_or_fetch_cst   : xxx_fetch AO__atomic_or_fetch   Z.lor.
-  Axiom wp_atom_nand_fetch_cst : xxx_fetch AO__atomic_nand_fetch nand.
+  Axiom wp_atom_add_fetch_cst  : xxx_fetch "__atomic_add_fetch"  Z.add.
+  Axiom wp_atom_sub_fetch_cst  : xxx_fetch "__atomic_sub_fetch"  Z.sub.
+  Axiom wp_atom_and_fetch_cst  : xxx_fetch "__atomic_and_fetch"  Z.land.
+  Axiom wp_atom_xor_fetch_cst  : xxx_fetch "__atomic_xor_fetch"  Z.lxor.
+  Axiom wp_atom_or_fetch_cst   : xxx_fetch "__atomic_or_fetch"   Z.lor.
+  Axiom wp_atom_nand_fetch_cst : xxx_fetch "__atomic_nand_fetch" nand.
 
   (** Derived AU1 specs *)
 
@@ -451,7 +451,7 @@ Section with_Σ.
     forall memorder acc_type p Q,
       [| memorder = _SEQ_CST |] **
       atom_load_cst_AU1 acc_type p Q
-      |-- wp_atom' AO__atomic_load_n acc_type [p; memorder] Q.
+      |-- wp_atom' "__atomic_load_n" acc_type [p; memorder] Q.
   Proof.
     intros. rewrite -wp_atom_load_cst.
     iIntros "[$ AU]".
@@ -471,7 +471,7 @@ Section with_Σ.
       [| memorder = _SEQ_CST |] **
       [| has_type_prop v acc_type |] **
       atom_store_cst_AU1 acc_type p Q v
-      |-- wp_atom' AO__atomic_store_n acc_type [p; memorder; v] Q.
+      |-- wp_atom' "__atomic_store_n" acc_type [p; memorder; v] Q.
   Proof.
     intros. rewrite -wp_atom_store_cst.
     iIntros "[$ [$ AU]]".
@@ -490,7 +490,7 @@ Section with_Σ.
       [| memorder = _SEQ_CST |] **
       [| has_type_prop v acc_type |] **
       atom_exchange_n_cst_AU1 acc_type p Q v
-      |-- wp_atom' AO__atomic_exchange_n acc_type [p; memorder; v] Q.
+      |-- wp_atom' "__atomic_exchange_n" acc_type [p; memorder; v] Q.
   Proof.
     intros. rewrite -wp_atom_exchange_n_cst.
     iIntros "[$ [$ AU]]".
